chore: CLAUDE: refactor some names; Claude seems to be better than I am at picking names IMHO. Might be closer to Mathlib conventions.

Traat/criticalpairs.lean
@@ -43,56 +43,56 @@ def Position.get? (p : Position) (t : Term) : Option Term :=
 abbrev Position.head : Position := []
 
 @[simp, grind .]
-lemma varValidHead (h : p.valid (var x)) : p = Position.head := by
+lemma Position.eq_head_of_valid_var (h : p.valid (var x)) : p = Position.head := by
   revert h; induction p <;> grind [Position.valid]
 
 @[simp, grind .]
-lemma funcValidHead (h : p.valid (func x)) : p = Position.head := by
+lemma Position.eq_head_of_valid_func (h : p.valid (func x)) : p = Position.head := by
   revert h; induction p <;> grind [Position.valid]
 
 
-lemma Position.validSubst {p : Position} {t : Term} (σ : Subst)
+lemma Position.valid_apply {p : Position} {t : Term} (σ : Subst)
   (h : p.valid t)
   : p.valid <| t.apply σ := by
   match p, t with
   | [], _ => simp [valid]
   | left::ps, t₁ @@ t₂ =>
-    simp [apply, valid]; apply Position.validSubst
+    simp [apply, valid]; apply Position.valid_apply
     . simp [valid] at h; trivial
   | right::ps, t₁ @@ t₂ =>
-    simp [apply, valid]; apply Position.validSubst
+    simp [apply, valid]; apply Position.valid_apply
     . simp [valid] at h; trivial
   | _::_, var _ => simp [valid] at h
   | _::_, func _ => simp [valid] at h
 
-lemma validAppend {p₁ p₂ : Position} (h : (p₁++p₂).valid t)
+lemma Position.valid_append_left {p₁ p₂ : Position} (h : (p₁++p₂).valid t)
   : p₁.valid t := by
   revert h
   match p₁, t with
   | [], _ => simp [Position.valid]
-  | left::_, t₁ @@ _ => simp [Position.valid]; intro h; apply validAppend h
-  | right::_, _ @@ t₂ => simp [Position.valid]; intro h; apply validAppend h
+  | left::_, t₁ @@ _ => simp [Position.valid]; intro h; apply Position.valid_append_left h
+  | right::_, _ @@ t₂ => simp [Position.valid]; intro h; apply Position.valid_append_left h
   | _::_, var _ => simp [Position.valid]
   | _::_, func _ => simp [Position.valid]
 
-lemma validAppendTail {p₁ p₂ : Position} (h : (p₁++p₂).valid t)
-  : p₂.valid <| p₁.get t (validAppend h) := by
+lemma Position.valid_append_right {p₁ p₂ : Position} (h : (p₁++p₂).valid t)
+  : p₂.valid <| p₁.get t (Position.valid_append_left h) := by
   revert h
   match p₁, t with
   | [], _ => simp [Position.valid, Position.get]
-  | left::_, t₁ @@ _ => simp [Position.valid, Position.get]; intro h; apply validAppendTail h
-  | right::_, _ @@ t₂ => simp [Position.valid, Position.get]; intro h; apply validAppendTail h
+  | left::_, t₁ @@ _ => simp [Position.valid, Position.get]; intro h; apply Position.valid_append_right h
+  | right::_, _ @@ t₂ => simp [Position.valid, Position.get]; intro h; apply Position.valid_append_right h
   | _::_, var _ => simp [Position.valid]
   | _::_, func _ => simp [Position.valid]
 
 @[simp]
-lemma getAppend {p₁ p₂ : Position} (h : (p₁++p₂).valid t)
-  : (p₁ ++ p₂).get t h = p₂.get (p₁.get t <| validAppend h) (validAppendTail h) := by
+lemma Position.get_append {p₁ p₂ : Position} (h : (p₁++p₂).valid t)
+  : (p₁ ++ p₂).get t h = p₂.get (p₁.get t <| Position.valid_append_left h) (Position.valid_append_right h) := by
   revert h
   match p₁, t with
   | [], _ => simp [Position.valid, Position.get]
-  | left::_, t₁ @@ _ => simp [Position.valid, Position.get]; intro h; apply getAppend h
-  | right::_, _ @@ t₂ => simp [Position.valid, Position.get]; intro h; apply getAppend h
+  | left::_, t₁ @@ _ => simp [Position.valid, Position.get]; intro h; apply Position.get_append h
+  | right::_, _ @@ t₂ => simp [Position.valid, Position.get]; intro h; apply Position.get_append h
   | _::_, var _ => simp [Position.valid]
   | _::_, func _ => simp [Position.valid]
 
@@ -111,35 +111,35 @@ def Position.splitOnSubst (p : Position) (t : Term) (σ : Subst) : Position × P
   | [], _ => ([], [])
 
 @[simp]
-lemma splitOnSubstHead : Position.splitOnSubst [] t σ = ([], []) := by
+lemma Position.splitOnSubst_head : Position.splitOnSubst [] t σ = ([], []) := by
   induction t <;> simp [Position.splitOnSubst]
 
-lemma splitOnSubstValid {p : Position} (h : p.valid (t.apply σ))
+lemma Position.splitOnSubst_fst_valid {p : Position} (h : p.valid (t.apply σ))
   : (p.splitOnSubst t σ).fst |>.valid t := by
   revert h
   match p, t with
   | [], _ => simp [Position.valid]
   | left::p', t₁ @@ _ =>
     simp [Position.splitOnSubst, apply, Position.valid]
-    intros; apply splitOnSubstValid; grind
+    intros; apply Position.splitOnSubst_fst_valid; grind
   | right::p', _ @@ t₂ =>
     simp [Position.splitOnSubst, apply, Position.valid]
-    intros; apply splitOnSubstValid; grind
+    intros; apply Position.splitOnSubst_fst_valid; grind
   | _, var _ =>
     simp [Position.valid, Position.splitOnSubst, apply]
   | _, func _ =>
     simp [Position.valid, Position.splitOnSubst, apply]
 
-lemma splitOnSubstConcat {p : Position}
+lemma Position.splitOnSubst_concat {p : Position}
  : (p.splitOnSubst t σ).1 ++ (p.splitOnSubst t σ).2 = p := by
   match p, t with
   | [], _ => simp
   | left::p', t₁ @@ _ =>
     simp [Position.splitOnSubst]
-    apply splitOnSubstConcat
+    apply Position.splitOnSubst_concat
   | right::p', _ @@ t₂ =>
     simp [Position.splitOnSubst]
-    apply splitOnSubstConcat
+    apply Position.splitOnSubst_concat
   | _, var _ =>
     simp [Position.splitOnSubst]
   | _, func _ =>
@@ -151,7 +151,7 @@ def IsOuterPosition (p : Position) (t : Term) (σ : Subst) : Bool :=
   let ⟨p, _⟩ := p.splitOnSubst t σ
   if h : (p.valid t) then p.get t h |>.isVar else false
 
-lemma isOuterSplit (h : IsOuterPosition p t σ) :
+lemma IsOuterPosition.exists_split (h : IsOuterPosition p t σ) :
   ∃ (p₁ p₂ : Position) (x : Var) (h₁ : p₁.valid t),
     p = p₁ ++ p₂ ∧ p₁.get t h₁ = var x := by
   revert h t
@@ -192,22 +192,22 @@ match p, t with
 | _::_, var _ => by simp [Position.valid] at h
 | _::_, func _ => by simp [Position.valid] at h
 
-lemma validSubstAt {p : Position} (h : p.valid t)
+lemma Term.substAt_valid_aux {p : Position} (h : p.valid t)
   : p.valid (t.substAt p h u) := by
   revert h
   match p, t with
   | [], _ => simp [Position.valid]
   | left::p', t₁ @@ _ =>
     simp [Position.valid, substAt]
-    apply validSubstAt
+    apply Term.substAt_valid_aux
   | right::p', _ @@ t₂ =>
     simp [Position.valid, substAt]
-    apply validSubstAt
+    apply Term.substAt_valid_aux
   | _::_, var _ => simp [Position.valid, substAt]
   | _::_, func _ => simp [Position.valid, substAt]
 
 @[simp]
-lemma getSubstAt' {t : Term} {p : Position}
+lemma Position.get_substAt_of_valid {t : Term} {p : Position}
  (h : p.valid t)
  (h' : p.valid (t.substAt p h u))
  : p.get (t.substAt p h u) h' = u := by
@@ -216,15 +216,15 @@ lemma getSubstAt' {t : Term} {p : Position}
   | [], _ => simp [Position.valid, substAt, Position.get]
   | left::p', t₁ @@ _ =>
     simp [Position.valid, substAt, substAt]
-    apply getSubstAt'
+    apply Position.get_substAt_of_valid
   | right::p', _ @@ t₂ =>
     simp [Position.valid, substAt, substAt]
-    apply getSubstAt'
+    apply Position.get_substAt_of_valid
   | _::_, var _ => simp [Position.valid, substAt]
   | _::_, func _ => simp [Position.valid, substAt]
 
-lemma getSubstAt {t : Term} {p : Position} (h : p.valid t)
- : p.get (t.substAt p h u) (validSubstAt h) = u := by
+lemma Position.get_substAt {t : Term} {p : Position} (h : p.valid t)
+ : p.get (t.substAt p h u) (Term.substAt_valid_aux h) = u := by
  simp
 
 def Position.Inc (p q : Position) : Bool :=
@@ -240,15 +240,15 @@ instance Position.instHasSubset : HasSubset Position where
   Subset p q := Position.Inc p q
 
 @[simp]
-lemma subsetHead {p : Position} : [] ⊆ p := by
+lemma Position.empty_subset {p : Position} : [] ⊆ p := by
   simp [Subset, Position.Inc]
 
 @[simp]
-lemma subsetNotHead {p : Position} : ¬ m::p ⊆ [] := by
+lemma Position.not_cons_subset_empty {p : Position} : ¬ m::p ⊆ [] := by
   simp [Subset, Position.Inc]
 
 @[simp]
-lemma subsetTail {p q : Position} : (m::p ⊆ m::q) = (p ⊆ q) := by
+lemma Position.cons_subset_cons_iff {p q : Position} : (m::p ⊆ m::q) = (p ⊆ q) := by
   cases m
   . match p, q with
     | [], _ => simp [Subset, Position.Inc]
@@ -262,23 +262,23 @@ lemma subsetTail {p q : Position} : (m::p ⊆ m::q) = (p ⊆ q) := by
     | _, _ => simp [Subset, Position.Inc]
 
 @[grind .]
-lemma subsetNotTail {p q : Position} (h : m ≠ n) : ¬ (m::p ⊆ n::q) := by
+lemma Position.not_cons_subset_cons_of_ne {p q : Position} (h : m ≠ n) : ¬ (m::p ⊆ n::q) := by
   revert h
   cases m <;> cases n <;> simp [Subset, Position.Inc]
 
 -- A little tedium here
 @[grind →]
-lemma validInc {p q : Position} (h : q.valid t) (inc : p ⊆ q)
+lemma Position.valid_of_valid_of_subset {p q : Position} (h : q.valid t) (inc : p ⊆ q)
  : p.valid t := by
   revert inc h; simp [Subset]
   match p, q, t with
   | [], _, _ => simp [Position.valid]
   | left::p', left::q', t₁ @@ _ =>
     simp [Position.valid, Position.Inc]
-    apply validInc
+    apply Position.valid_of_valid_of_subset
   | right::p', right::q', _ @@ t₂ =>
     simp [Position.valid, Position.Inc]
-    apply validInc
+    apply Position.valid_of_valid_of_subset
   | _, _::_, var _ => simp [Position.valid]
   | _, _::_, func _ => simp [Position.valid]
   | _::_, [], _ => simp [Position.Inc]
@@ -299,27 +299,27 @@ instance Position.instSDiff : SDiff Position where
   sdiff := Position.sdiff
 
 @[simp]
-lemma sdiffHead₁ {p : Position} : p \ [] = p := by
-  induction p <;> simp [sdiff, Position.sdiff]
+lemma Position.sdiff_empty_right {p : Position} : p \ [] = p := by
+  induction p <;> simp [SDiff.sdiff, Position.sdiff]
 
 @[simp]
-lemma sdiffHead₂ {p : Position} : [] \ p = [] := by
-  induction p <;> simp [sdiff, Position.sdiff]
+lemma Position.empty_sdiff {p : Position} : [] \ p = [] := by
+  induction p <;> simp [SDiff.sdiff, Position.sdiff]
 
 @[simp]
-lemma sdiffCons {p q : Position} {m : Move} : (m::p) \ (m::q) = p \ q := by
-  cases m <;> simp [sdiff, Position.sdiff]
+lemma Position.sdiff_cons_cons {p q : Position} {m : Move} : (m::p) \ (m::q) = p \ q := by
+  cases m <;> simp [SDiff.sdiff, Position.sdiff]
 
 @[simp]
-lemma sdiffEmpty {p : Position} : (p \ p) = [] := by
+lemma Position.sdiff_self {p : Position} : (p \ p) = [] := by
   induction p <;> simp; trivial
 
-lemma sdiffSum {p q : Position} (inc : p ⊆ q) : q = p ++ (q \ p) := by
+lemma Position.eq_append_sdiff_of_subset {p q : Position} (inc : p ⊆ q) : q = p ++ (q \ p) := by
   revert inc
   cases p <;> cases q <;> simp
   case cons.cons m _ n _ =>
     by_cases h:(m = n)
-    . simp [h]; apply sdiffSum
+    . simp [h]; apply Position.eq_append_sdiff_of_subset
     . grind
 
 def Position.IsOrtho (p q : Position) : Bool :=
@@ -333,35 +333,35 @@ def Position.IsOrtho (p q : Position) : Bool :=
 infix:50 " ⊥ " => Position.IsOrtho
 
 @[grind =]
-lemma isOrthoCons (h : m ≠ n) : (m::p) ⊥ (n::q) := by
+lemma Position.isOrtho_cons_of_ne (h : m ≠ n) : (m::p) ⊥ (n::q) := by
   revert h; cases m <;> cases n <;> simp [Position.IsOrtho]
 
 @[simp]
-lemma isOrthoCons' : ((m::p) ⊥ (m::q)) = (p ⊥ q) := by
+lemma Position.isOrtho_cons_iff : ((m::p) ⊥ (m::q)) = (p ⊥ q) := by
   cases m <;> simp only [Position.IsOrtho]
 
 @[grind .]
-lemma isOrthoNil : ¬ ([] ⊥ p) := by
+lemma Position.not_isOrtho_nil_left : ¬ ([] ⊥ p) := by
   cases p <;> simp [Position.IsOrtho]
 
 @[grind .]
-lemma isOrthoNil' : ¬ (p ⊥ []) := by
+lemma Position.not_isOrtho_nil_right : ¬ (p ⊥ []) := by
   cases p <;> simp [Position.IsOrtho]
 
-lemma trichotomy (p q : Position) : p ⊆ q ∨ q ⊆ p ∨ p ⊥ q := by
+lemma Position.trichotomy (p q : Position) : p ⊆ q ∨ q ⊆ p ∨ p ⊥ q := by
   cases p <;> cases q <;> try simp
   case cons.cons m _ n _ =>
     by_cases h:(m = n)
-    . simp [h]; apply trichotomy
+    . simp [h]; apply Position.trichotomy
     . grind
 
-lemma commOrth {p q : Position} (h : p ⊥ q) : q ⊥ p := by
+lemma Position.isOrtho_comm {p q : Position} (h : p ⊥ q) : q ⊥ p := by
   revert h
   match p, q with
   | [], _ => simp [Position.IsOrtho]
   | _::_, [] => simp [Position.IsOrtho]
-  | left::_, left::_ => simp [Position.IsOrtho]; apply commOrth
-  | right::_, right::_ => simp [Position.IsOrtho]; apply commOrth
+  | left::_, left::_ => simp [Position.IsOrtho]; apply Position.isOrtho_comm
+  | right::_, right::_ => simp [Position.IsOrtho]; apply Position.isOrtho_comm
   | left::_, right::_ => simp [Position.IsOrtho]
   | right::_, left::_ => simp [Position.IsOrtho]
 
@@ -373,7 +373,7 @@ open Position Move Term
 #print Rules
 #print Rule
 
--- This is a compbination of `Reduces.subst` and `Reduces.ax`.
+-- This is a compbination of `Reduces.apply` and `Reduces.ax`.
 @[simp]
 def Rule.matchesHead (r : Rule) (t : Term) (σ : Subst) : Prop :=
   r.lhs.apply σ = t
@@ -395,7 +395,7 @@ def Rule.rewriteAt
 
 -- This is our master theorem to move between the "nice" definition of rewriting to the
 -- position based one, which will allow us to do horrible reasoning about critical pairs.
-theorem rewriteIsRewriteAt {ℛ : Rules} (t t' : RTerm ℛ) (red : t ~> t')
+theorem Reduces.exists_rewriteAt {ℛ : Rules} (t t' : RTerm ℛ) (red : t ~> t')
  : ∃ r ∈ ℛ, ∃ (p : Position) (σ : Subst) (h : p.valid t),
   r.matchesAt t p σ h ∧ t' = r.rewriteAt t p σ h := by
   simp [Red.reduces] at red
@@ -420,21 +420,21 @@ theorem rewriteIsRewriteAt {ℛ : Rules} (t t' : RTerm ℛ) (red : t ~> t')
     trivial
 
 @[simp]
-lemma substValid {t : Term} {p : Position}
+lemma Term.substAt_valid {t : Term} {p : Position}
   (h : p.valid t)
   : p.valid (t.substAt p h u) := by
   revert h
   match p, t with
   | [], _ => simp [valid]
-  | left::_, _ @@ _ => simp [valid, substAt]; apply substValid
-  | right::_, _ @@ _ => simp [valid, substAt]; apply substValid
+  | left::_, _ @@ _ => simp [valid, substAt]; apply Term.substAt_valid
+  | right::_, _ @@ _ => simp [valid, substAt]; apply Term.substAt_valid
   | left::_, var _ => simp [valid]
   | right::_, var _ => simp [valid]
   | left::_, func _ => simp [valid]
   | right::_, func _ => simp [valid]
 
 -- A subtitution at an orthogonal position does not change validity
-lemma orthValidL {p q : Position} (h₁ : p.valid t) (h₂ : q.valid t) (orth : p ⊥ q) :
+lemma Position.valid_substAt_of_ortho_left {p q : Position} (h₁ : p.valid t) (h₂ : q.valid t) (orth : p ⊥ q) :
   p.valid (t.substAt q h₂ u) := by
   revert h₁ h₂ orth
   match p, q, t with
@@ -442,12 +442,12 @@ lemma orthValidL {p q : Position} (h₁ : p.valid t) (h₂ : q.valid t) (orth : 
   | _, [], _ => grind
   | m::p', n::q', t₁ @@ t₂ =>
     cases m <;> cases n <;> simp [valid, substAt] <;> try grind
-    . apply orthValidL
-    . apply orthValidL
+    . apply Position.valid_substAt_of_ortho_left
+    . apply Position.valid_substAt_of_ortho_left
   | _::_, _::_, var _ => grind
   | _::_, _::_, func _ => grind
 
-lemma orthValidR {p q : Position} (h₁ : p.valid t) (h₂ : q.valid t) (orth : p ⊥ q) :
+lemma Position.valid_substAt_of_ortho_right {p q : Position} (h₁ : p.valid t) (h₂ : q.valid t) (orth : p ⊥ q) :
   q.valid (t.substAt p h₁ u) := by
   revert h₁ h₂ orth
   match p, q, t with
@@ -455,12 +455,12 @@ lemma orthValidR {p q : Position} (h₁ : p.valid t) (h₂ : q.valid t) (orth : 
   | _, [], _ => grind
   | m::p', n::q', t₁ @@ t₂ =>
     cases m <;> cases n <;> simp [valid, substAt] <;> try grind
-    . apply orthValidR
-    . apply orthValidR
+    . apply Position.valid_substAt_of_ortho_right
+    . apply Position.valid_substAt_of_ortho_right
   | _::_, _::_, var _ => grind
   | _::_, _::_, func _ => grind
 
-lemma substAtgetOrth' {p q : Position}
+lemma Position.get_substAt_of_ortho_aux {p q : Position}
   (h₁ : p.valid t)
   (h₂ : q.valid t)
   (orth : p ⊥ q)
@@ -476,22 +476,22 @@ lemma substAtgetOrth' {p q : Position}
     simp [Position.get, Term.substAt]
   | left::_, left::_, _ @@ _ =>
     simp [IsOrtho, Position.get, Term.substAt]
-    intros; apply substAtgetOrth'; grind
+    intros; apply Position.get_substAt_of_ortho_aux; grind
   | right::_, right::_, _ @@ _ =>
     simp [IsOrtho, Position.get, Term.substAt]
-    intros; apply substAtgetOrth'; grind
+    intros; apply Position.get_substAt_of_ortho_aux; grind
   | _::_, _::_, var _ => simp [valid]
   | _::_, _::_, func _ => simp [valid]
 
 
-lemma substAtgetOrth {p q : Position}
+lemma Position.get_substAt_of_ortho {p q : Position}
   (h₁ : p.valid t)
   (h₂ : q.valid t)
   (orth : p ⊥ q)
-  : q.get (t.substAt p h₁ u) (orthValidR h₁ h₂ orth) = q.get t h₂ := by
-  grind [substAtgetOrth']
+  : q.get (t.substAt p h₁ u) (Position.valid_substAt_of_ortho_right h₁ h₂ orth) = q.get t h₂ := by
+  grind [Position.get_substAt_of_ortho_aux]
 
-lemma substOrth'
+lemma Term.substAt_comm_of_ortho_aux
   {p q : Position}
   (t u₁ u₂ : Term)
   (h₁ : p.valid t)
@@ -507,33 +507,33 @@ lemma substOrth'
   | _, [], _ => grind
   | m::p', n::q', t₁ @@ t₂ =>
     cases m <;> cases n <;> simp [valid, substAt] <;> intros
-    . apply substOrth'; trivial
-    . apply substOrth'; trivial
+    . apply Term.substAt_comm_of_ortho_aux; trivial
+    . apply Term.substAt_comm_of_ortho_aux; trivial
   | _::_, _::_, var _ => grind
   | _::_, _::_, func _ => grind
 
-lemma substOrth
+lemma Term.substAt_comm_of_ortho
   {p q : Position}
   (t u₁ u₂ : Term)
   (h₁ : p.valid t)
   (h₂ : q.valid t)
   (orth : p ⊥ q)
-  : (t.substAt p h₁ u₁).substAt q (orthValidR h₁ h₂ orth) u₂ =
-    (t.substAt q h₂ u₂).substAt p (orthValidL h₁ h₂ orth) u₁ := by
-  grind [substOrth']
+  : (t.substAt p h₁ u₁).substAt q (Position.valid_substAt_of_ortho_right h₁ h₂ orth) u₂ =
+    (t.substAt q h₂ u₂).substAt p (Position.valid_substAt_of_ortho_left h₁ h₂ orth) u₁ := by
+  grind [Term.substAt_comm_of_ortho_aux]
 
 -- rewriting at orthogonal positions commutes
 -- FIXME: rename this
-lemma rewriteAtOrthCom
+lemma Rule.rewriteAt_comm_of_ortho
   {ru₁ ru₂ : Rule}
   {p q : Position}
   (t : RTerm ℛ)
   (h₁ : p.valid t)
   (h₂ : q.valid t)
   (orth : p ⊥ q)
-  : ru₂.rewriteAt (ru₁.rewriteAt t p σ h₁) q τ (orthValidR h₁ h₂ orth) =
-    ru₁.rewriteAt (ru₂.rewriteAt t q τ h₂) p σ (orthValidL h₁ h₂ orth) := by
-  grind [Rule.rewriteAt, substOrth]
+  : ru₂.rewriteAt (ru₁.rewriteAt t p σ h₁) q τ (Position.valid_substAt_of_ortho_right h₁ h₂ orth) =
+    ru₁.rewriteAt (ru₂.rewriteAt t q τ h₂) p σ (Position.valid_substAt_of_ortho_left h₁ h₂ orth) := by
+  grind [Rule.rewriteAt, Term.substAt_comm_of_ortho]
 
 -- Basically, if `rw₁` happens at the root, and `rw₂` happens
 -- beneath a leaf of the lhs, then
@@ -554,7 +554,7 @@ def varPos (t : Term) (x : Var) : List Position :=
   | t₁ @@ t₂ => Position.join (varPos t₁ x) (varPos t₂ x)
 
 @[grind .]
-lemma isValidVarPos : ∀ p ∈ varPos t x, p.valid t := by
+lemma Position.valid_of_mem_varPos : ∀ p ∈ varPos t x, p.valid t := by
   induction t <;> simp [varPos, valid]
   case _ t₁ t₂ ih₁ ih₂ =>
     intros p shape
@@ -563,7 +563,7 @@ lemma isValidVarPos : ∀ p ∈ varPos t x, p.valid t := by
     . rw [← h₂]; simp [valid]; grind
 
 @[grind →]
-lemma isVarVarPos'
+lemma Position.get_eq_var_of_mem_varPos_aux
   (p : Position)
   (mem : p ∈ varPos t x)
   (h : p.valid t)
@@ -579,11 +579,11 @@ lemma isVarVarPos'
     . rw [← h₂]; simp [valid, Position.get]; grind
     . rw [← h₂]; simp [valid, Position.get]; grind
 
-lemma isVarVarPos {p : Position} (mem : p ∈ varPos t x)
-  : p.get t (isValidVarPos p mem) = var x := by
-  grind [isVarVarPos']
+lemma Position.get_eq_var_of_mem_varPos {p : Position} (mem : p ∈ varPos t x)
+  : p.get t (Position.valid_of_mem_varPos p mem) = var x := by
+  grind [Position.get_eq_var_of_mem_varPos_aux]
 
-lemma varPosComplete {p : Position} {h : p.valid t}
+lemma Position.mem_varPos_of_get_eq_var {p : Position} {h : p.valid t}
   (isVar : p.get t h = var x) : p ∈ varPos t x := by
   revert p
   induction t
@@ -599,7 +599,7 @@ lemma varPosComplete {p : Position} {h : p.valid t}
       cases hd <;> simp [Position.get, varPos] <;> grind
 
 -- Sheesh this is awkward
-lemma orthLeaf
+lemma Position.ortho_leaf
   (h₁ : p.valid t) (h₂ : q.valid t)
   (isVar₁ : p.get t h₁ |>.isVar)
   (isVar₂ : q.get t h₂ |>.isVar)
@@ -609,52 +609,52 @@ lemma orthLeaf
   | right::_, left::_, t₁ @@ t₂ => grind
   | right::_, right::_, t₁ @@ t₂ =>
     simp; simp [Position.get] at isVar₁; simp [Position.get] at isVar₂; simp at neq
-    apply orthLeaf (t:=t₂) <;> trivial
+    apply Position.ortho_leaf (t:=t₂) <;> trivial
   | left::_, left::_, t₁ @@ t₂ =>
     simp; simp [Position.get] at isVar₁; simp [Position.get] at isVar₂; simp at neq
-    apply orthLeaf (t:=t₁) <;> trivial
+    apply Position.ortho_leaf (t:=t₁) <;> trivial
   | [], [], _ => grind
   | _::_, [], t₁ @@ t₂ => simp [isVar, Position.get] at isVar₂
   | [], _::_, t₁ @@ t₂ => simp [isVar, Position.get] at isVar₁
   | [], _ :: _, var _ => simp [valid] at h₂
 
-lemma orthVarPos : ∀ p ∈ varPos t x, ∀ q ∈ varPos t x, p ≠ q → p ⊥ q := by
-  intros p mem₁ q mem₂ neq; apply orthLeaf <;> try trivial
-  . rw [isVarVarPos']
+lemma Position.ortho_varPos : ∀ p ∈ varPos t x, ∀ q ∈ varPos t x, p ≠ q → p ⊥ q := by
+  intros p mem₁ q mem₂ neq; apply Position.ortho_leaf <;> try trivial
+  . rw [Position.get_eq_var_of_mem_varPos_aux]
     . simp [isVar]
     . trivial
     . grind
-  . rw [isVarVarPos']
+  . rw [Position.get_eq_var_of_mem_varPos_aux]
     . simp [isVar]
     . trivial
     . grind
 
 -- We used to need this now it's just for free...
-lemma nodupVarPos : (varPos t x).Nodup := by
+lemma varPos_nodup : (varPos t x).Nodup := by
   cases t <;> simp [varPos]
   . grind
   . rw [List.nodup_append]
     constructor
     . rw [List.nodup_map_iff (f := fun l => left::l)]
-      . apply nodupVarPos
+      . apply varPos_nodup
       . simp
     . constructor
       . rw [List.nodup_map_iff (f := fun l => right::l)]
-        . apply nodupVarPos
+        . apply varPos_nodup
         . simp
       . simp only [List.mem_map,
          ne_eq, forall_exists_index, and_imp, forall_apply_eq_imp_iff₂,
          List.cons.injEq, reduceCtorEq, false_and, not_false_eq_true,
          implies_true] -- holy crap
 
-lemma substValidList {p : Position} {ps : List Position}
+lemma Term.substAt_valid_list {p : Position} {ps : List Position}
   (h : p.valid t)
   (h' : ∀ q ∈ ps, q.valid t)
   (orth : ∀ q ∈ ps, p ≠ q → p ⊥ q)
   (mem : q ∈ ps)
   : q.valid (t.substAt p h u) := by
   by_cases eq:(q = p); simp [eq]
-  grind [orthValidR]
+  grind [Position.valid_substAt_of_ortho_right]
 
 def Term.substAll (t u : Term) (ps : List Position)
   (h : ∀ p ∈ ps, p.valid t)
@@ -666,7 +666,7 @@ def Term.substAll (t u : Term) (ps : List Position)
     Term.substAll
       (t.substAt p (by grind) u)
       u ps'
-      (by grind [substValidList])
+      (by grind [Term.substAt_valid_list])
       (by grind)
 
 -- Need some algebraic fact about `(t₁ @@ t₂).substAll u (varPos (t₁ @@ t₂) x)`.
@@ -699,8 +699,8 @@ private lemma substAllAppDecomp {ps₁ ps₂ : List Position}
     simp [join, substAll, substAt]
     apply ih -- again, proof irrelevance
 
-theorem substAllIsVarSubst (t u : Term) (x : Var) :
-  t.substAll u (varPos t x) isValidVarPos orthVarPos =
+theorem Term.substAll_eq_varSubst (t u : Term) (x : Var) :
+  t.substAll u (varPos t x) Position.valid_of_mem_varPos Position.ortho_varPos =
   t.apply (varSubst x u) := by
   induction t
   case _ y =>
@@ -711,10 +711,10 @@ theorem substAllIsVarSubst (t u : Term) (x : Var) :
     simp [varPos, apply]
     rw [substAllAppDecomp] -- now we pay the piper for all those hyps
     . congr
-    . apply isValidVarPos
-    . apply isValidVarPos
-    . apply orthVarPos
-    . apply orthVarPos
+    . apply Position.valid_of_mem_varPos
+    . apply Position.valid_of_mem_varPos
+    . apply Position.ortho_varPos
+    . apply Position.ortho_varPos
 
 -- Since orthogonal substs commute, inserting a subst into the list is the same as doing it first
 
@@ -725,16 +725,16 @@ theorem substAllIsVarSubst (t u : Term) (x : Var) :
 -- same as rewriting all at once. Then prove that a rewrite at any position is the same as
 -- rewriting at some element of the `varPos` list.
 
-lemma substAtIdem {t : Term}
+lemma Term.substAt_idem {t : Term}
   (h : p.valid t)
   (h' : p.valid (t.substAt p h u)) -- this can be proven
   : (t.substAt p h u).substAt p h' u = t.substAt p h u := by
   match p, t with
   | [], _ => simp [substAt]
-  | left::_, _@@_ => simp [substAt]; apply substAtIdem
-  | right::_, _@@_ => simp [substAt]; apply substAtIdem
+  | left::_, _@@_ => simp [substAt]; apply Term.substAt_idem
+  | right::_, _@@_ => simp [substAt]; apply Term.substAt_idem
 
-lemma rewriteAtIsRewrite {t : RTerm ℛ}
+lemma Rule.rewriteAt_is_reduce {t : RTerm ℛ}
   {mem : ru ∈ ℛ}
   (h : p.valid t)
   (mtch : ru.matchesAt t p σ h)
@@ -748,29 +748,29 @@ lemma rewriteAtIsRewrite {t : RTerm ℛ}
   | left::p', t₁ @@ _ =>
     simp [Rule.matchesAt, Position.get, Rule.rewriteAt, substAt]
     intro mtch; apply Reduces.congrLeft
-    apply rewriteAtIsRewrite <;> trivial
+    apply Rule.rewriteAt_is_reduce <;> trivial
   | right::p', _ @@ t₂ =>
     simp [Rule.matchesAt, Position.get, Rule.rewriteAt, substAt]
     intro mtch; apply Reduces.congrRight
-    apply rewriteAtIsRewrite <;> trivial
+    apply Rule.rewriteAt_is_reduce <;> trivial
 
 @[simp]
 def RTerm.substAt (t : RTerm ℛ) (p : Position) (h : p.valid t) (u : Term) : RTerm ℛ :=
   Term.substAt t p h u
 
 @[simp]
-lemma substAtGet' : substAt t p h (p.get t h') = t := by
+lemma Term.get_substAt_of_valid : substAt t p h (p.get t h') = t := by
   revert h h'
   match p, t with
   | [], _ => simp [valid, substAt, Position.get]
-  | left::_ , _@@_ => simp [valid, substAt, Position.get]; apply substAtGet'
-  | right::_ , _@@_ => simp [valid, substAt, Position.get]; apply substAtGet'
+  | left::_ , _@@_ => simp [valid, substAt, Position.get]; apply Term.get_substAt_of_valid
+  | right::_ , _@@_ => simp [valid, substAt, Position.get]; apply Term.get_substAt_of_valid
   | _::_, var _ => simp [valid]
   | _::_, func _ => simp [valid]
 
-lemma substAtGet : substAt t p h (p.get t h) = t := by simp
+lemma Term.get_substAt : substAt t p h (p.get t h) = t := by simp
 
-lemma rewriteSubstAt
+lemma Rule.rewriteAt_substAt
   {t u₁ u₂ : RTerm ℛ}
   {p : Position}
   (h : p.valid t)
@@ -782,28 +782,28 @@ lemma rewriteSubstAt
     simp [substAt]; grind
   | left::p', t₁ @@ _ =>
     simp [Term.substAt, valid]; intros
-    apply Reduces.congrLeft; apply rewriteSubstAt; grind
+    apply Reduces.congrLeft; apply Rule.rewriteAt_substAt; grind
   | right::p', _ @@ t₂ =>
     simp [Term.substAt, valid]; intros
-    apply Reduces.congrRight; apply rewriteSubstAt; grind
+    apply Reduces.congrRight; apply Rule.rewriteAt_substAt; grind
   | _::_, var _ => simp [valid]
   | _::_, func _ => simp [valid]
 
-lemma rewriteSubstAt'
+lemma Rule.rewriteAt_substAt_aux
   {t u₁ u₂ : RTerm ℛ}
   {p : Position}
   (h : p.valid t)
   (getAt : p.get t h = u₁)
   (red : u₁ ~> u₂)
   : t ~> t.substAt p h u₂ := by
-    have h' := substAtGet (h:=h)
-    have h'' := rewriteSubstAt h red
+    have h' := Term.get_substAt (h:=h)
+    have h'' := Rule.rewriteAt_substAt h red
     rw [getAt] at h'
     rw [RTerm.substAt, h'] at h''
     trivial
 
 -- A no-op substitution is a rewrite
-lemma rewriteAtIsRewrite' {t : RTerm ℛ}
+lemma Rule.rewriteAt_is_reduce_aux {t : RTerm ℛ}
   {_ : ru ∈ ℛ}
   (h : p.valid t)
   (idem : p.get t h = ru.rhs.apply σ)
@@ -813,9 +813,9 @@ lemma rewriteAtIsRewrite' {t : RTerm ℛ}
   rw [← eq]
   apply refl_trans_clos.refl
 
-#check substOrth'
+#check Term.substAt_comm_of_ortho_aux
 
-lemma substAllSwap {t : Term}
+lemma Term.substAll_swap {t : Term}
   (orth : p ⊥ q)
   (allValid₁ : ∀ p' ∈ p::q::ps, p'.valid t)
   (allOrth₁ : ∀ p' ∈ p::q::ps, ∀ p'' ∈ p::q::ps, p' ≠ p'' → p' ⊥ p'')
@@ -825,9 +825,9 @@ lemma substAllSwap {t : Term}
     t.substAll u (q::p::ps) allValid₂ allOrth₂ := by
   simp [substAll]
   congr 1
-  apply substOrth'; grind
+  apply Term.substAt_comm_of_ortho_aux; grind
 
-lemma substAllIdem {t : Term}
+lemma Term.substAll_idem {t : Term}
   (h₁ : ∀ p' ∈ ps, p'.valid t)
   (h₂ : ∀ p' ∈ p::ps, p'.valid t)
   (orth₁ : ∀ p' ∈ ps, ∀ p'' ∈ ps, p' ≠ p'' → p' ⊥ p'')
@@ -839,19 +839,19 @@ lemma substAllIdem {t : Term}
   case _ => simp at mem
   case _ hd tail ih =>
     by_cases h:(p = hd)
-    . simp [h, substAll, substAtIdem]
+    . simp [h, substAll, Term.substAt_idem]
     . intros
       have h' : p ⊥ hd := by grind
-      rw [substAllSwap] <;> try grind
+      rw [Term.substAll_swap] <;> try grind
       . simp [substAll]
         apply ih <;> try grind
         . simp; constructor
-          . apply orthValidL <;> grind
-          . grind [substValidList]
+          . apply Position.valid_substAt_of_ortho_left <;> grind
+          . grind [Term.substAt_valid_list]
 
-#check substAtgetOrth
+#check Position.get_substAt_of_ortho
 
-lemma rewriteAtSubstAllStutter {ℛ : Rules} {t u₁ u₂ : RTerm ℛ}
+lemma Rule.rewriteAt_substAll_stutter {ℛ : Rules} {t u₁ u₂ : RTerm ℛ}
   (allValid : ∀ p ∈ ps, p.valid t)
   (mtch : ∀ p (mem : p ∈ ps),
     p.get t (allValid p mem) = u₁ ∨ p.get t (allValid p mem) = u₂)
@@ -868,26 +868,26 @@ lemma rewriteAtSubstAllStutter {ℛ : Rules} {t u₁ u₂ : RTerm ℛ}
     case _ hl =>
       apply refl_trans_clos.step
        (b := t.substAt p (by grind) u₂)
-      . apply rewriteSubstAt'; trivial; grind
+      . apply Rule.rewriteAt_substAt_aux; trivial; grind
       . apply ih
         intros q mem
         by_cases eq:(p = q)
         . simp [eq]
         . have pq_orth : p ⊥ q := by grind
           simp
-          rw [substAtgetOrth] <;> try grind
+          rw [Position.get_substAt_of_ortho] <;> try grind
     case _ getEq =>
-      rewrite (occs := .pos [1]) [← substAtGet (t:=t) (p:=p)]
+      rewrite (occs := .pos [1]) [← Term.get_substAt (t:=t) (p:=p)]
       rw [getEq]
       apply ih
       . intros q mem
         by_cases eq:(p = q)
         . simp [eq]
         . have pq_orth : p ⊥ q := by grind
-          rw [substAtgetOrth] <;> try grind
+          rw [Position.get_substAt_of_ortho] <;> try grind
       . grind
 
-lemma rewriteAtSubstAll {ℛ : Rules}
+lemma Rule.rewriteAt_substAll {ℛ : Rules}
   {t u₁ u₂ : RTerm ℛ}
   {p : Position}
   (mem' : p ∈ ps)
@@ -897,29 +897,29 @@ lemma rewriteAtSubstAll {ℛ : Rules}
   (red : u₁ ~> u₂)
   : t.substAt p (allValid p mem') u₂ ~>*
   t.substAll u₂ ps allValid allOrth := by
-  rw [← substAllIdem (p := p) ] <;> try grind
+  rw [← Term.substAll_idem (p := p) ] <;> try grind
   simp [substAll]
-  apply rewriteAtSubstAllStutter
+  apply Rule.rewriteAt_substAll_stutter
   . intros q mem
     by_cases eq:(p = q)
     . simp [eq]
     . have pq_orth : p ⊥ q := by grind
-      rw [substAtgetOrth] <;> try grind
+      rw [Position.get_substAt_of_ortho] <;> try grind
       . left; apply mtch; trivial
   . trivial
 
 #print Subst.join
 
 -- Ok this is slightly too weak
-#check substAllIsVarSubst
+#check Term.substAll_eq_varSubst
 
-#check isValidVarPos
+#check Position.valid_of_mem_varPos
 
 def Subst.replace (σ : Subst) (x : Var) (u : Term) : Subst :=
   fun y => if y = x then u else σ y
 
-lemma substAllIsReplace (t u : Term) (x : Var) :
-  (t.apply τ).substAll u (varPos t x) (by grind [isValidVarPos, validSubst]) orthVarPos =
+lemma Term.substAll_eq_substAt (t u : Term) (x : Var) :
+  (t.apply τ).substAll u (varPos t x) (by grind [Position.valid_of_mem_varPos, Position.valid_apply]) Position.ortho_varPos =
   t.apply (τ.replace x u) := by
   induction t
   case _ y =>
@@ -930,25 +930,25 @@ lemma substAllIsReplace (t u : Term) (x : Var) :
     simp [varPos, apply]
     rw [substAllAppDecomp] -- now we pay the piper for all those hyps
     . congr
-    . intros; grind [isValidVarPos, validSubst]
-    . intros; grind [isValidVarPos, validSubst]
-    . apply orthVarPos
-    . apply orthVarPos
+    . intros; grind [Position.valid_of_mem_varPos, Position.valid_apply]
+    . intros; grind [Position.valid_of_mem_varPos, Position.valid_apply]
+    . apply Position.ortho_varPos
+    . apply Position.ortho_varPos
 
-#check rewriteAtSubstAll
+#check Rule.rewriteAt_substAll
 
-lemma getSubst {p : Position}
+lemma Position.get_apply {p : Position}
   (h : p.valid t)
   (h' : p.valid (t.apply σ))
   : p.get (t.apply σ) h' = (p.get t h).apply σ := by
   match p, t with
   | [], _ => simp [Position.get]
-  | left::_, t₁ @@ _ => simp [apply, Position.get]; apply getSubst
-  | right::_, _ @@ t₂ => simp [apply, Position.get]; apply getSubst
+  | left::_, t₁ @@ _ => simp [apply, Position.get]; apply Position.get_apply
+  | right::_, _ @@ t₂ => simp [apply, Position.get]; apply Position.get_apply
   | _::_, var _ => simp [valid] at h
   | _::_, func _ => simp [valid] at h
 
-lemma rewriteAtVarIsSubst
+lemma Rule.rewriteAt_var_eq_subst
   {ℛ : Rules}
   {t u₁ u₂ : RTerm ℛ}
   {p : Position}
@@ -956,23 +956,23 @@ lemma rewriteAtVarIsSubst
   (h' : p.get t h = var x)
   (mtch : τ x = u₁)
   (rew : u₁ ~> u₂)
-  : (t.apply τ).substAt p (validSubst τ h) u₂ ~>*
+  : (t.apply τ).substAt p (Position.valid_apply τ h) u₂ ~>*
     t.apply (τ.replace x u₂) := by
   simp [RTerm.apply]
-  rw [← substAllIsReplace t u₂ x (τ := τ)]
+  rw [← Term.substAll_eq_substAt t u₂ x (τ := τ)]
   -- Notations smotations
-  have h₂ := rewriteAtSubstAll
+  have h₂ := Rule.rewriteAt_substAll
    (t := t.apply τ) (u₁ := u₁) (u₂ := u₂) (p := p) (ps := varPos t x)
   simp at h₂
   apply h₂
-  . apply varPosComplete <;> grind
-  . intros; rw [getSubst]
-    . rw [isVarVarPos']
+  . apply Position.mem_varPos_of_get_eq_var <;> grind
+  . intros; rw [Position.get_apply]
+    . rw [Position.get_eq_var_of_mem_varPos_aux]
       . simp [apply]; trivial
       . trivial
     . grind
   . trivial
-  . grind [isValidVarPos, validSubst]
+  . grind [Position.valid_of_mem_varPos, Position.valid_apply]
 
 structure PreCriticalPair (ℛ : Rules) where
   r₁ : Rule
@@ -984,24 +984,24 @@ structure PreCriticalPair (ℛ : Rules) where
   p : Position
   valid_p : p.valid r₁.lhs
   nvar_p : ¬ (p.get r₁.lhs valid_p |>.isVar)
-  mtch₂ : r₂.matchesAt (r₁.lhs.apply σ₁) p σ₂ (validSubst σ₁ valid_p)
+  mtch₂ : r₂.matchesAt (r₁.lhs.apply σ₁) p σ₂ (Position.valid_apply σ₁ valid_p)
 
 def PreCriticalPair.joins {ℛ : Rules} (cp : PreCriticalPair ℛ) : Prop :=
   let lhs : RTerm ℛ := cp.r₁.rhs.apply cp.σ₁
   let rhs : RTerm ℛ := cp.r₁.lhs.apply cp.σ₁
                          |>.substAt cp.p
-                          (validSubst cp.σ₁ cp.valid_p)
+                          (Position.valid_apply cp.σ₁ cp.valid_p)
                           (cp.r₂.rhs.apply cp.σ₂)
   lhs ~>*.*<~ rhs
 
-#check rewriteIsRewriteAt
-#check trichotomy
+#check Reduces.exists_rewriteAt
+#check Position.trichotomy
 
-#check rewriteAtOrthCom
-#check rewriteAtIsRewrite
-#check substAtgetOrth'
+#check Rule.rewriteAt_comm_of_ortho
+#check Rule.rewriteAt_is_reduce
+#check Position.get_substAt_of_ortho_aux
 
-lemma joinableOrth (t : RTerm ℛ)
+lemma joinable_of_ortho (t : RTerm ℛ)
   (ru₁ ru₂ : Rule)
   (mem₁ : ru₁ ∈ ℛ)
   (mem₂ : ru₂ ∈ ℛ)
@@ -1013,62 +1013,62 @@ lemma joinableOrth (t : RTerm ℛ)
   (mtch₂ : ru₂.matchesAt t p₂ σ₂ h₂)
   (orth : p₁ ⊥ p₂)
    : ru₁.rewriteAt t p₁ σ₁ h₁ ~>*.*<~ ru₂.rewriteAt t p₂ σ₂ h₂ := by
-  exists ru₂.rewriteAt (ru₁.rewriteAt t p₁ σ₁ h₁) p₂ σ₂ (orthValidR h₁ h₂ orth)
+  exists ru₂.rewriteAt (ru₁.rewriteAt t p₁ σ₁ h₁) p₂ σ₂ (Position.valid_substAt_of_ortho_right h₁ h₂ orth)
   apply And.intro
   . apply refl_trans_clos.step _ _ _ _ (by apply refl_trans_clos.refl)
-    apply rewriteAtIsRewrite; trivial
+    apply Rule.rewriteAt_is_reduce; trivial
     simp [Rule.rewriteAt, Rule.matchesAt]
-    rw [substAtgetOrth']
+    rw [Position.get_substAt_of_ortho_aux]
     . apply mtch₂
     . trivial
     . trivial
   . apply refl_trans_clos.step _ _ _ _ (by apply refl_trans_clos.refl)
-    rw [rewriteAtOrthCom] <;> try trivial
-    apply rewriteAtIsRewrite; trivial
+    rw [Rule.rewriteAt_comm_of_ortho] <;> try trivial
+    apply Rule.rewriteAt_is_reduce; trivial
     simp [Rule.rewriteAt, Rule.matchesAt]
-    rw [substAtgetOrth']
+    rw [Position.get_substAt_of_ortho_aux]
     . apply mtch₁
     . trivial
-    . apply commOrth; trivial
+    . apply Position.isOrtho_comm; trivial
 
 #print PreCriticalPair
 
-lemma matchesAtHeadIsInst {t : Term} {ru : Rule}
+lemma Rule.matchesAt_head_iff {t : Term} {ru : Rule}
   (h : ru.matchesAt t [] σ (Eq.refl true))
   : t = ru.lhs.apply σ := by
   revert h
   simp [Rule.matchesAt, Position.get]
   grind
 
-#check isOuterSplit
-#check rewriteAtVarIsSubst
-#check splitOnSubstConcat
+#check IsOuterPosition.exists_split
+#check Rule.rewriteAt_var_eq_subst
+#check Position.splitOnSubst_concat
 #print substAt
 
-lemma validConcat {p₁ p₂ : Position}
+lemma Position.valid_append {p₁ p₂ : Position}
   (h : (p₁ ++ p₂).valid t)
   : p₁.valid t := by
   revert h
   match p₁, t with
   | [], _ => simp [valid]
-  | left::_, _ @@ _ => simp [valid]; apply validConcat
-  | right::_, _ @@ _ => simp [valid]; apply validConcat
+  | left::_, _ @@ _ => simp [valid]; apply Position.valid_append
+  | right::_, _ @@ _ => simp [valid]; apply Position.valid_append
   | _::_, var _ => simp [valid]
   | _::_, func _ => simp [valid]
 
-lemma validConcatGet {p₁ p₂ : Position}
+lemma Position.valid_appendGet {p₁ p₂ : Position}
   (h₁ : (p₁ ++ p₂).valid t)
   (h₂ : p₁.valid t)
   : p₂.valid (p₁.get t h₂) := by
   revert h₁ h₂
   match p₁, t with
   | [], _ => simp [valid, Position.get]
-  | left::_, _ @@ _ => simp [valid]; apply validConcatGet
-  | right::_, _ @@ _ => simp [valid]; apply validConcatGet
+  | left::_, _ @@ _ => simp [valid]; apply Position.valid_appendGet
+  | right::_, _ @@ _ => simp [valid]; apply Position.valid_appendGet
   | _::_, var _ => simp [valid]
   | _::_, func _ => simp [valid]
 
-lemma substConcat {p₁ p₂ : Position}
+lemma Term.substAt_append {p₁ p₂ : Position}
   (h₁ : p₁.valid t)
   (h₂ : p₂.valid (p₁.get t h₁))
   (h₃ : (p₁ ++ p₂).valid t)
@@ -1076,12 +1076,12 @@ lemma substConcat {p₁ p₂ : Position}
   revert h₁
   match p₁, t with
   | [], _ => simp [Position.get, substAt]
-  | left::_, _ @@ _ => simp [substAt, Position.get]; intros; apply substConcat
-  | right::_, _ @@ _ => simp [substAt, Position.get]; intros; apply substConcat
+  | left::_, _ @@ _ => simp [substAt, Position.get]; intros; apply Term.substAt_append
+  | right::_, _ @@ _ => simp [substAt, Position.get]; intros; apply Term.substAt_append
   | _::_, var _ => simp [valid]
   | _::_, func _ => simp [valid]
 
-lemma matchesConcat {p₁ p₂ : Position} {ru : Rule}
+lemma Rule.matchesAt_append {p₁ p₂ : Position} {ru : Rule}
   (h₁ : p₁.valid t)
   (h₂ : p₂.valid (p₁.get t h₁))
   (h₃ : (p₁ ++ p₂).valid t)
@@ -1090,10 +1090,10 @@ lemma matchesConcat {p₁ p₂ : Position} {ru : Rule}
   revert mtchConcat
   simp [Rule.matchesAt]
 
-#check rewriteAtIsRewrite
-#check rewriteAtVarIsSubst
+#check Rule.rewriteAt_is_reduce
+#check Rule.rewriteAt_var_eq_subst
 
-lemma rewriteReplace {t : RTerm ℛ}
+lemma Rule.rewriteAt_replace {t : RTerm ℛ}
   (rewAt : let u' : RTerm ℛ := σ x; u' ~> u)
   : t.apply σ ~>* t.apply (σ.replace x u) := by
   induction t
@@ -1108,7 +1108,7 @@ lemma rewriteReplace {t : RTerm ℛ}
   case _ => simp [apply]; apply refl_trans_clos.refl
   case _ =>
     simp [apply]
-    apply Reduces.congReflTrans <;> trivial
+    apply Reduces.refl_trans_clos_congr <;> trivial
 
 lemma IsNotOuterValid {p : Position}
   (h : p.valid <| t.apply σ)
@@ -1158,7 +1158,7 @@ lemma IsNotOuterNvar
   (isNOuter : ¬ IsOuterPosition p t σ)
   : ¬ (p.get t h |>.isVar) := by simp; apply IsNotOuterNvar_aux <;> trivial
 
-lemma joinableTop (t : RTerm ℛ)
+lemma joinable_of_top (t : RTerm ℛ)
   (joinable : ∀ cp : PreCriticalPair ℛ, cp.joins)
   (ru₁ ru₂ : Rule)
   (mem₁ : ru₁ ∈ ℛ)
@@ -1172,44 +1172,44 @@ lemma joinableTop (t : RTerm ℛ)
   by_cases isOuter:(IsOuterPosition p₂ ru₁.lhs σ₁)
   -- This case is awkward: though we're rewriting *at* `p₂` (with `rewriteAt`)
   -- we want to consider a rewrite at a higher position, that of a variable
-  -- in `ru₁.lhs`, so we can apply `rewriteAtVarIsSubst`.
+  -- in `ru₁.lhs`, so we can apply `Rule.rewriteAt_var_eq_subst`.
   -- This is not a head rewrite though.
-  . have ⟨p₁, ⟨p₂', ⟨x, ⟨h, ⟨h', h''⟩⟩⟩⟩⟩ := isOuterSplit isOuter
+  . have ⟨p₁, ⟨p₂', ⟨x, ⟨h, ⟨h', h''⟩⟩⟩⟩⟩ := IsOuterPosition.exists_split isOuter
     revert mtch₂ isOuter h₂; rw [h']; intros h₂ mtch₂ isOuter
     simp [Rule.rewriteAt]
-    have h₁₁ : p₁.valid t := by apply validConcat; trivial
-    have h₁₂ : p₂'.valid (p₁.get t h₁₁) := by apply validConcatGet; trivial
-    rw [substConcat (t:=t) (h₁ := h₁₁) (h₂ := h₁₂)]
+    have h₁₁ : p₁.valid t := by apply Position.valid_append; trivial
+    have h₁₂ : p₂'.valid (p₁.get t h₁₁) := by apply Position.valid_appendGet; trivial
+    rw [Term.substAt_append (t:=t) (h₁ := h₁₁) (h₂ := h₁₂)]
     let u : RTerm ℛ := (p₁.get t h₁₁).substAt p₂' h₁₂ (ru₂.rhs.apply σ₂)
     let u_l : RTerm ℛ := σ₁ x
     have h₅ : σ₁ x = p₁.get t h₁₁ := by
       calc
         σ₁ x = (var x).apply σ₁ := by simp [apply]
         _    = (p₁.get ru₁.lhs h).apply σ₁ := by rw [← h'']
-        _    = (p₁.get (ru₁.lhs.apply σ₁) (validSubst σ₁ h)) := by rw [getSubst]
+        _    = (p₁.get (ru₁.lhs.apply σ₁) (Position.valid_apply σ₁ h)) := by rw [Position.get_apply]
         _    = (p₁.get t h₁₁) := by congr
     have u_rew : u_l ~> u := by -- This is the most finicky proof I have ever done
       simp [Rule.matchesAt] at mtch₂
       have h₃ : p₂'.valid u_l := by
         simp [Rule.matchesAt, Position.get] at mtch₁
         simp [u_l]
-        have h₄ := validAppendTail h₂
+        have h₄ := Position.valid_append_right h₂
         rw [h₅]; trivial
       simp [u_l, u]; rw [h₅]
-      apply rewriteAtIsRewrite <;> trivial
+      apply Rule.rewriteAt_is_reduce <;> trivial
     exists (ru₁.rhs.apply (σ₁.replace x u))
     apply And.intro
-    . apply rewriteReplace; trivial
+    . apply Rule.rewriteAt_replace; trivial
     . have h₆ :
        substAt t p₁ h₁₁ ((p₁.get t h₁₁).substAt p₂' h₁₂ (ru₂.rhs.apply σ₂)) =
        substAt t p₁ h₁₁ u := by trivial
       rw [h₆]
       -- Very annoying
       let u' : RTerm ℛ := ru₁.lhs.apply (σ₁.replace x u)
-      apply refl_trans_clos_transitive (y := u')
+      apply refl_trans_clos_trans (y := u')
       simp [Rule.matchesAt, Position.get] at mtch₁
       simp [← mtch₁]; simp [u']
-      . apply rewriteAtVarIsSubst <;> trivial
+      . apply Rule.rewriteAt_var_eq_subst <;> trivial
       . simp [u']
         apply refl_trans_clos.step _ _ _ _ (by apply refl_trans_clos.refl)
         simp [Red.reduces]; apply Reduces.head
@@ -1231,19 +1231,19 @@ lemma joinableTop (t : RTerm ℛ)
     simp [← mtch₁]
     apply joins
 
-lemma congrJoinL {t₁ t₂ u : RTerm ℛ}
+lemma joins_congr_left {t₁ t₂ u : RTerm ℛ}
   (joins : t₁ ~>*.*<~ t₂)
   : (t₁ @@@ u) ~>*.*<~ (t₂ @@@ u) := by
   have ⟨t', _⟩ := joins
-  exists (t' @@@ u); grind [Reduces.congReflTransL]
+  exists (t' @@@ u); grind [Reduces.refl_trans_clos_congr_left]
 
-lemma congrJoinR {t u₁ u₂ : RTerm ℛ}
+lemma joins_congr_right {t u₁ u₂ : RTerm ℛ}
   (joins : u₁ ~>*.*<~ u₂)
   : (t @@@ u₁) ~>*.*<~ (t @@@ u₂) := by
   have ⟨u', _⟩ := joins
-  exists (t @@@ u'); grind [Reduces.congReflTransR]
+  exists (t @@@ u'); grind [Reduces.refl_trans_clos_congr_right]
 
-lemma joinableInc (t : RTerm ℛ)
+lemma joinable_mono (t : RTerm ℛ)
   (joinable : ∀ cp : PreCriticalPair ℛ, cp.joins)
   (ru₁ ru₂ : Rule)
   (mem₁ : ru₁ ∈ ℛ)
@@ -1258,7 +1258,7 @@ lemma joinableInc (t : RTerm ℛ)
    : ru₁.rewriteAt t p₁ σ₁ h₁ ~>*.*<~ ru₂.rewriteAt t p₂ σ₂ h₂ := by
   match p₁, p₂ with
   | [], _ =>
-    have h := joinableTop (ru₁:=ru₁) (ru₂:=ru₂) (t:=t)
+    have h := joinable_of_top (ru₁:=ru₁) (ru₂:=ru₂) (t:=t)
     simp [Rule.rewriteHead] at h
     simp [Rule.rewriteAt, substAt]
     apply h <;> trivial
@@ -1268,16 +1268,16 @@ lemma joinableInc (t : RTerm ℛ)
     case _ => simp [valid] at h₁
     case _ =>
       simp [Rule.rewriteAt, substAt]
-      apply congrJoinL
-      apply joinableInc <;> trivial
+      apply joins_congr_left
+      apply joinable_mono <;> trivial
   | right::p₁', right::p₂' =>
     cases t
     case _ => simp [valid] at h₁
     case _ => simp [valid] at h₁
     case _ =>
       simp [Rule.rewriteAt, substAt]
-      apply congrJoinR
-      apply joinableInc <;> trivial
+      apply joins_congr_right
+      apply joinable_mono <;> trivial
   | left::p₁', right::p₂' => simp [Subset, Inc] at inc
   | right::p₁', left::p₂' => simp [Subset, Inc] at inc
 
@@ -1290,12 +1290,12 @@ theorem PreCritJoinableWC {ℛ : Rules}
   : weakly_confluent (termRed ℛ) := by
   simp [weakly_confluent]
   intros t u₁ u₂ red₁ red₂
-  have ⟨ru₁, ⟨mem₁, ⟨p₁, ⟨σ₁,⟨h₁, ⟨mtch₁, rew₁⟩⟩⟩⟩⟩⟩ := rewriteIsRewriteAt _ _ red₁
-  have ⟨ru₂, ⟨mem₂, ⟨p₂, ⟨σ₂,⟨h₂, ⟨mtch₂, rew₂⟩⟩⟩⟩⟩⟩ := rewriteIsRewriteAt _ _ red₂
-  rcases trichotomy p₁ p₂ with h | h | h
-  . rw [rew₁, rew₂]; apply joinableInc <;> grind
-  . rw [rew₁, rew₂]; apply swap_joins; apply joinableInc <;> grind
-  . rw [rew₁, rew₂]; apply joinableOrth <;> grind
+  have ⟨ru₁, ⟨mem₁, ⟨p₁, ⟨σ₁,⟨h₁, ⟨mtch₁, rew₁⟩⟩⟩⟩⟩⟩ := Reduces.exists_rewriteAt _ _ red₁
+  have ⟨ru₂, ⟨mem₂, ⟨p₂, ⟨σ₂,⟨h₂, ⟨mtch₂, rew₂⟩⟩⟩⟩⟩⟩ := Reduces.exists_rewriteAt _ _ red₂
+  rcases Position.trichotomy p₁ p₂ with h | h | h
+  . rw [rew₁, rew₂]; apply joinable_mono <;> grind
+  . rw [rew₁, rew₂]; apply joins_comm; apply joinable_mono <;> grind
+  . rw [rew₁, rew₂]; apply joinable_of_ortho <;> grind
 
 #print Finset.map
 #print Var
@@ -1330,7 +1330,7 @@ def freshVarInv (renamed : Var) (avoid : Finset Var) : Var :=
 #check String.length_append
 #check Finset.max'_eq_iff
 
-lemma freshVarNotIn
+lemma freshVar_not_mem
   : freshVar x S ∉ S := by
   simp [freshVar]
   by_cases h:(S.Nonempty) <;> simp [h]
@@ -1354,32 +1354,32 @@ lemma freshVarNotIn
 #check String.toList_ofList
 #check List.toString
 
-lemma freshVarInvInv :
+lemma freshVar_inv_inv :
   freshVarInv (freshVar x S) S = x := by
   simp [freshVar, freshVarInv]
   by_cases h:S.Nonempty <;> simp [h]
 
-lemma freshVarDistinct
+lemma freshVar_distinct
   (neq : x ≠ y)
   : freshVar x S ≠ freshVar y S := by
   intro h
   have h' : freshVarInv (freshVar x S) S = freshVarInv (freshVar y S) S := by grind
-  grind [freshVarInvInv]
+  grind [freshVar_inv_inv]
 
 def Subst.ren (avoid : Finset Var) : Subst := fun x => var <| freshVar x avoid
 
 #print Subst.scomp
-#check Subst.scompApply
+#check Subst.scomp_apply
 
 def Subst.joinAvoiding (σ₁ : Subst) (σ₂ : Subst) (S : Finset Var) : Subst :=
   fun x => if x ∈ S then σ₂ x else σ₁ (freshVarInv x S)
 
-lemma joinAvoidingApply₁ (σ₁ : Subst) (σ₂ : Subst)
+lemma Subst.join_apply_left (σ₁ : Subst) (σ₂ : Subst)
   : (Subst.ren S).scomp (σ₁.joinAvoiding σ₂ S) = σ₁ := by
   funext x; simp [Subst.scomp, Subst.ren, apply, Subst.joinAvoiding]
-  simp [freshVarNotIn, freshVarInvInv]
+  simp [freshVar_not_mem, freshVar_inv_inv]
 
-lemma joinAvoidingApply₂ {t : Term} {σ₁ σ₂ : Subst}
+lemma Subst.join_apply_right {t : Term} {σ₁ σ₂ : Subst}
   {S : Finset Var}
   (h : t.vars ⊆ S)
   : t.apply (σ₁.joinAvoiding σ₂ S) = t.apply σ₂ := by
@@ -1391,24 +1391,24 @@ lemma joinAvoidingApply₂ {t : Term} {σ₁ σ₂ : Subst}
 
 
 -- FIXME: is this the right lemma?
-lemma matchUnifies {t₁ t₂ : Term}
+lemma Rule.matches_unifies {t₁ t₂ : Term}
   (h : t₁.apply σ₁ = t₂.apply σ₂)
   (h' : t₂.vars ⊆ S)
   : Unifier (σ₁.joinAvoiding σ₂ S) (t₁.apply <| Subst.ren S) t₂ := by
   simp [Unifier]
-  rw [← Subst.scompApply]
-  simp [joinAvoidingApply₁]
-  rw [joinAvoidingApply₂] <;> grind
+  rw [← Subst.scomp_apply]
+  simp [Subst.join_apply_left]
+  rw [Subst.join_apply_right] <;> grind
 
 
-lemma matchUnify {t₁ t₂ : Term}
+lemma Rule.match_unify {t₁ t₂ : Term}
   (h : t₁.apply σ₁ = t₂.apply σ₂)
   (_ : t₂.vars ⊆ S)
   : Unify (t₁.apply <| Subst.ren S) t₂ := by
   exists σ₁.joinAvoiding σ₂ S
-  apply matchUnifies <;> trivial
+  apply Rule.matches_unifies <;> trivial
 
-#check unifyComplete
+#check unify_complete
 
 
 structure CriticalPair (ℛ : Rules) where
@@ -1431,28 +1431,28 @@ def CriticalPair.joins (cp : CriticalPair ℛ) : Prop :=
   let lhs : RTerm ℛ := cp.ru₁.rhs.apply (Subst.ren avoids) |>.apply mgu
   let rhs : RTerm ℛ :=
     (cp.ru₁.lhs.apply (Subst.ren avoids) |>.apply mgu).substAt cp.p
-    (validSubst mgu (validSubst (Subst.ren avoids) cp.valid_p))
+    (Position.valid_apply mgu (Position.valid_apply (Subst.ren avoids) cp.valid_p))
     (cp.ru₂.rhs.apply mgu)
   lhs ~>*.*<~ rhs
 
 lemma UnifySymm  (h : Unify t u) : Unify u t := by
   rcases h with ⟨σ, _⟩
-  exists σ; apply unifierSymm; trivial
+  exists σ; apply Unifier.symm; trivial
 
 #print PreCriticalPair
 
-lemma unifCritIsSome
+lemma unif_crit_isSome
   (cp : PreCriticalPair ℛ)
   : (unify ((cp.p.get cp.r₁.lhs cp.valid_p).apply (Subst.ren <| cp.r₂.lhs.vars ∪ cp.r₂.rhs.vars))
             cp.r₂.lhs).isSome := by
-  apply unifyProgress
-  apply matchUnifies
+  apply unify_progress
+  apply Rule.matches_unifies
   . have h := cp.mtch₂
     simp [Rule.matchesAt] at h
-    rw [← getSubst, h]
+    rw [← Position.get_apply, h]
   . simp
 
-def criticalOfPreCritical (cp : PreCriticalPair ℛ) : CriticalPair ℛ :=
+def critical_of_preCritical (cp : PreCriticalPair ℛ) : CriticalPair ℛ :=
   CriticalPair.mk
     cp.r₁
     cp.r₂
@@ -1460,74 +1460,74 @@ def criticalOfPreCritical (cp : PreCriticalPair ℛ) : CriticalPair ℛ :=
     cp.mem₂
     cp.p
     cp.valid_p
-    (unifCritIsSome cp)
+    (unif_crit_isSome cp)
 
-#check unifyComplete'
-#check Reduces.substTrans
+#check unify_complete'
+#check Reduces.refl_trans_clos_apply
 
 -- ugh
-lemma rwSubstApply
+lemma rewrite_apply_subst
   {t u : Term}
   {σ σ' : Subst}
   {p : Position}
   (h₁ : p.valid t)
   (h₃ : σ' = σ)
   (h₂ : p.valid (t.apply σ))
-  : (t.apply σ).substAt p h₂ u = (t.apply σ').substAt p (validSubst σ' h₁) u := by
+  : (t.apply σ).substAt p h₂ u = (t.apply σ').substAt p (Position.valid_apply σ' h₁) u := by
   symm at h₃
   congr
 
 -- can't believe I haven't needed this
-lemma substSubstAt {t u : Term}
+lemma Term.apply_substAt {t u : Term}
   (h : p.valid t)
   (h' : p.valid (t.apply σ))
   : (t.substAt p h u).apply σ = (t.apply σ).substAt p h' (u.apply σ) := by
   revert h h'
   match p, t with
   | [], _ => simp [substAt]
-  | left::_, _ @@ _ => simp [apply, substAt, valid]; apply substSubstAt
-  | right::_, _ @@ _ => simp [apply, substAt, valid]; apply substSubstAt
+  | left::_, _ @@ _ => simp [apply, substAt, valid]; apply Term.apply_substAt
+  | right::_, _ @@ _ => simp [apply, substAt, valid]; apply Term.apply_substAt
   | _::_, var _ => simp [valid]
   | _::_, func _ => simp [valid]
 
-lemma joinSubst {t u : RTerm ℛ}
+lemma joins_apply {t u : RTerm ℛ}
   (joins_t_u : t ~>*.*<~ u)
   : t.apply σ ~>*.*<~ u.apply σ := by
   have ⟨v, _⟩ := joins_t_u
   simp [joins]; exists (v.apply σ)
-  apply And.intro <;> apply Reduces.substTrans <;> grind
+  apply And.intro <;> apply Reduces.refl_trans_clos_apply <;> grind
 
 lemma JoinsCPImpJoinsPC
   (cp : PreCriticalPair ℛ)
-  (joins : (criticalOfPreCritical cp).joins)
+  (joins : (critical_of_preCritical cp).joins)
   : cp.joins := by
   cases cp
   case _ r₁ r₂ mem₁ mem₂ σ₁ σ₂ p valid_p nvar mtch =>
-  simp [criticalOfPreCritical, CriticalPair.joins] at joins
+  simp [critical_of_preCritical, CriticalPair.joins] at joins
   simp [PreCriticalPair.joins]
   simp [Rule.matchesAt] at mtch
-  have h := matchUnifies (σ₁:=σ₁) (σ₂:=σ₂) (t₁ := p.get r₁.lhs valid_p) (t₂ := r₂.lhs) (S := r₂.lhs.vars ∪ r₂.rhs.vars)
-            (by rw [← getSubst]; symm; trivial)
+  have h := Rule.matches_unifies (σ₁:=σ₁) (σ₂:=σ₂) (t₁ := p.get r₁.lhs valid_p) (t₂ := r₂.lhs) (S := r₂.lhs.vars ∪ r₂.rhs.vars)
+            (by rw [← Position.get_apply]; symm; trivial)
             (by simp)
-  have ⟨τ, isUnif⟩ := unifyComplete h
-  rw (occs:= .pos [1]) [← joinAvoidingApply₁ (σ₁:=σ₁) (σ₂:=σ₂) (S := r₂.lhs.vars ∪ r₂.rhs.vars)]
-  have h := joinAvoidingApply₂ (t:=r₂.rhs) (σ₁:=σ₁) (σ₂:=σ₂) (S := r₂.lhs.vars ∪ r₂.rhs.vars) (by simp)
+  have ⟨τ, isUnif⟩ := unify_complete h
+  rw (occs:= .pos [1]) [← Subst.join_apply_left (σ₁:=σ₁) (σ₂:=σ₂) (S := r₂.lhs.vars ∪ r₂.rhs.vars)]
+  have h := Subst.join_apply_right (t:=r₂.rhs) (σ₁:=σ₁) (σ₂:=σ₂) (S := r₂.lhs.vars ∪ r₂.rhs.vars) (by simp)
   rw [← h]
   rw [
-      rwSubstApply valid_p
-        (joinAvoidingApply₁ (σ₁:=σ₁) (σ₂:=σ₂) (S := r₂.lhs.vars ∪ r₂.rhs.vars))
+      rewrite_apply_subst valid_p
+        (Subst.join_apply_left (σ₁:=σ₁) (σ₂:=σ₂) (S := r₂.lhs.vars ∪ r₂.rhs.vars))
          (u:=(r₂.rhs.apply (σ₁.joinAvoiding σ₂ (r₂.lhs.vars ∪ r₂.rhs.vars))))]
-  simp [Subst.scompApply]
+  simp [Subst.scomp_apply]
   rw [isUnif]
-  simp [Subst.scompApply] -- horror!!!!
-  rw [← substSubstAt]
-  . apply joinSubst
+  simp [Subst.scomp_apply] -- horror!!!!
+  rw [← Term.apply_substAt]
+  . apply joins_apply
     trivial
 
 -- This is the main theorem: any failure to be locally confluent *must* come from
 -- a non-joinable critical pair.
 -- The converse is true as well, but we only state the "if" direction
-theorem criticalPairLemma {ℛ : Rules}
+theorem critical_pair_lemma {ℛ : Rules}
   (joinable : ∀ cp : CriticalPair ℛ, cp.joins)
   : weakly_confluent (termRed ℛ) := by
   apply PreCritJoinableWC
